theories/ValueOpts/ConstantPropagationSound.v
@@ -1,0 +1,125 @@
+Require Import CSet Le Coq.Classes.RelationClasses.
+
+Require Import Plus Util AllInRel Map Indexwise.
+Require Import CSet Val Var Env IL Sim Fresh Annotation LabelsDefined DecSolve OptionR.
+
+Require Import RenamedApart SetOperations Eqn Infra.Lattice WithTop ConstantPropagation.
+
+Set Implicit Arguments.
+Unset Printing Records.
+
+(* Constant Propagation *)
+
+Inductive isEqCmp : op -> Prop :=
+  IisEqCmp x c : isEqCmp (BinOp BinOpEq (Var x) (Con c)).
+
+Instance isEqCmp_dec e : Computable (isEqCmp e).
+Proof.
+  destruct e; try dec_solve.
+  destruct e1, e2; decide (b = BinOpEq); subst; try dec_solve.
+Defined.
+
+Definition getEqCmpVar (e:op) :=
+  match e with
+    | BinOp BinOpEq (Var x) (Con c) => x
+    | _ => default_var
+  end.
+
+Definition getEqCmpCon (e:op) :=
+  match e with
+    | BinOp BinOpEq (Var x) (Con c) => c
+    | _ => default_val
+  end.
+
+Definition aval2bool (v:aval) :=
+  match v with
+  | Some Top => Some Top
+  | Some (wTA v) => Some (wTA (val2bool v))
+  | _ => None
+  end.
+
+Lemma oval2bool_some v b
+: aval2bool v = Some (wTA b) ->
+  exists v', v = (Some (wTA v')) /\ val2bool v' = b.
+Proof.
+  destruct v; try destruct w; simpl; intros; inv H; eauto.
+Qed.
+
+Inductive cp_sound (AE:onv (withTop val)) :
+                     list (params*list aval)
+                     -> stmt
+                     -> ann bool
+                     -> Prop :=
+| CPOpr (x:var) Cp (b:bool) r e s
+  : cp_sound AE Cp s r
+    -> (b -> exp_eval AE e = AE x)
+    -> cp_sound AE Cp (stmtLet x e s) (ann1 b r)
+| CPIf Cp e (b:bool) s1 s2 (r1 r2:ann bool)
+       (Cond1:cp_sound AE Cp s1 r1)
+       (Cond2:cp_sound AE Cp s2 r2)
+  : cp_sound AE Cp (stmtIf e s1 s2) (ann2 b r1 r2)
+| CPGoto l Y Cp Z aY (b bf:bool)
+  : get Cp (counted l) (Z,aY)
+    -> length Z = length Y
+    -> (b -> PIR2 poLe (List.map (op_eval AE) Y) aY)
+    -> cp_sound AE Cp (stmtApp l Y) (ann0 b)
+| CPReturn Cp e b
+  : cp_sound AE Cp (stmtReturn e) (ann0 b)
+| CPLet Cp F t (b:bool) (rF:list (ann bool)) (r:ann bool) (rfLen:❬F❭=❬rF❭)
+  : (forall n Zs r,
+        get F n Zs ->
+        get rF n r ->
+        cp_sound AE (List.map (fun Zs => (fst Zs, lookup_list AE (fst Zs))) F ++ Cp) (snd Zs) r)
+    -> cp_sound AE (List.map (fun Zs => (fst Zs, lookup_list AE (fst Zs))) F ++ Cp) t r
+    -> cp_sound AE Cp (stmtFun F t) (annF b rF r).
+
+Definition indexwise_R1 {A} (P:A->Prop) LA :=
+forall n a, get LA n a -> P a.
+
+Definition indexwise_R1_dec {A} {P:A->Prop} LA (Rdec:(forall n a, get LA n a -> Computable (P a)))
+      : Computable (indexwise_R1 P LA).
+unfold Computable. revert LA Rdec. fix 1. intros LA Rdec.
+destruct LA; try now left; isabsurd.
+intros. destruct (Rdec 0 a).
+- eauto using get.
+- destruct (indexwise_R1_dec LA); clear indexwise_R1_dec; eauto using get.
+  + left. hnf; intros. inv H; eauto.
+  + right; intro HH. eapply n; hnf; intros; eapply HH; eauto using get.
+- right; intro HH. eapply n; hnf; intros; eapply HH; eauto using get.
+Defined.
+
+Instance cp_sound_dec AE ZL s r : Computable (cp_sound AE ZL s r).
+Proof.
+  hnf. revert AE ZL r; sind s; intros; destruct s; destruct r; try dec_solve.
+  - edestruct (IH s); eauto;
+      decide (a -> exp_eval AE e = AE x); try dec_solve;
+        try dec_solve.
+  - edestruct (IH s2 ltac:(eauto) AE ZL); eauto; [| dec_solve];
+      edestruct (IH s1 ltac:(eauto) AE ZL); eauto; [| dec_solve];
+        decide (op_eval AE e = None);
+        decide (aval2bool (op_eval AE e) = Some (wTA false));
+        (decide (poLe (Some (wTA val_false)) (op_eval AE e)));
+        decide (a); decide (getAnn r1); decide (getAnn r2); try dec_solve.
+  - destruct (get_dec ZL (counted l)) as [[[]]|]; try dec_solve.
+    decide (length l0 = length Y); try dec_solve.
+    decide (a -> PIR2 poLe (List.map (op_eval AE) Y) l1);
+      try dec_solve.
+  - assert (SZ:size s < size (stmtFun F s)) by eauto.
+    decide (❬F❭=❬sa❭); [|dec_solve].
+    edestruct (IH s SZ AE (List.map (fun Zs => (fst Zs, lookup_list AE (fst Zs))) F ++ ZL) r); [|dec_solve].
+    exploit (@indexwise_R2_dec _ _ (fun Zs r => cp_sound AE ((fun Zs0 : params * stmt => (fst Zs0,
+        lookup_list AE (fst Zs0))) ⊝ F ++ ZL) (snd Zs) r) F); eauto.
+    intros. eapply IH; eauto. destruct H; dec_solve.
+Defined.
+
+Definition cop2bool AE e := aval2bool (op_eval AE e).
+
+Lemma op_eval_cop2bool_not_none AE e
+  : op_eval AE e <> ⎣⎦
+    -> cop2bool AE e <> ⎣⎦.
+Proof.
+  unfold cop2bool, aval2bool; repeat cases; intros; eauto;
+    try congruence.
+Qed.
+
+Hint Resolve op_eval_cop2bool_not_none.
